\begin{frame}{课堂思考}
	\linespread{1.4}
	\begin{columns}
		\column{.5\textwidth}
			\begin{enumerate}
			  \item $y'=\df1{2x-y^2}$
			  \item $y'=\df{x}{x^2-y^2}$
			  \item $xy'=\sqrt{x^2-y^2}+y$
			  \item $y'=\df{3x^2+y^2-6x+3}{2xy-2y}$
			  \item $xy'+y=2\sqrt{xy}$
			  \item $xy'+y=y(\ln x+\ln y)$
			\end{enumerate}
		\column{.5\textwidth}
			\begin{enumerate}
			  \addtocounter{enumi}{6}
			  \item $xy'\ln x+y=\ln x+1$
			  \item $xy'\ln x+y=x(\ln x+1)$
			  \item $y'=\df y{2(\ln y-x)}$
			  \item $y'+x=\sqrt{x^2+y}$
			  \item $y'-\df yx=\df{2x}{3y^2}$
			  \item $2x\ln x\d y+y(y^2\ln x-1)\d x=0$
			\end{enumerate}
	\end{columns}
\end{frame}